expression_eval_smallstep.v
@@ -71,7 +71,7 @@ Lemma ehstep_expr_eval Γ ρ m1 m2 e1 e2 :
 Proof.
   destruct 1; inversion 1;
     by repeat match goal with
-    | H : is_pure (#{_} _) |- _ => inversion H; clear H
+    | H : is_pure (%#{_} _) |- _ => inversion H; clear H
     | _ => destruct (val_true_false_dec _ _) as [[[??]|[??]]|[??]]
     | _ => progress simplify_option_equality
     end || solve_elem_of.
